chore: refactor KmsUtils out to KeyStore

AwsCryptographicMaterialProviders/dafny/AwsCryptographyKeyStore/src/KmsUtils.dfy
@@ -1,14 +1,14 @@
 // Copyright Amazon.com Inc. or its affiliates. All Rights Reserved.
 // SPDX-License-Identifier: Apache-2.0
-include "../Model/AwsCryptographyKeyStoreAdminTypes.dfy"
-include "MutationStateStructures.dfy"
+include "../Model/AwsCryptographyKeyStoreTypes.dfy"
+include "KMSKeystoreOperations.dfy"
+include "KmsArn.dfy"
 
 module {:options "/functionSyntax:4" } KmsUtils {
   import opened Wrappers
   import KMS = Com.Amazonaws.Kms
   import KMSKeystoreOperations
   import KeyStoreTypes = KMSKeystoreOperations.Types
-  import Types = AwsCryptographyKeyStoreAdminTypes
   import KmsArn
 
   datatype KMSTuple = | KMSTuple(
@@ -69,26 +69,6 @@ module {:options "/functionSyntax:4" } KmsUtils {
     }
   }
 
-  datatype InternalSystemKey =
-    | TrustStorage()
-    | KmsSymEnc(
-        nameonly Tuple: KMSTuple,
-        nameonly KeyId: KMS.Types.KeyIdType
-      )
-  {
-    ghost predicate ValidState()
-    {
-      match this
-      case TrustStorage() => true
-      case KmsSymEnc(Tuple, KeyId) =>
-        && Tuple.ValidState()
-        && KMS.Types.IsValid_KeyIdType(KeyId)
-        && Tuple.Modifies == Tuple.Modifies
-    }
-    ghost const Modifies := match this
-      case TrustStorage() => {}
-      case KmsSymEnc(Tuple, KeyId) => Tuple.Modifies
-  }
 
   function ExtractKmsOpaque(
     error: KMSKeystoreOperations.KmsError
@@ -128,16 +108,6 @@ module {:options "/functionSyntax:4" } KmsUtils {
     }
   }
 
-  function KmsSymmetricKeyArnToKMSConfiguration(
-    kmsSymmetricArn: Types.KmsSymmetricKeyArn
-  ): (output: KeyStoreTypes.KMSConfiguration)
-    requires
-      match kmsSymmetricArn
-      case KmsKeyArn(arn) => KmsArn.ValidKmsArn?(arn)
-  {
-    match kmsSymmetricArn
-    case KmsKeyArn(kmsKeyArn) => KeyStoreTypes.kmsKeyArn(kmsKeyArn)
-  }
 
   predicate IsSupportedKeyManagerStrategy(
     terminalHierarchyVersion: KeyStoreTypes.HierarchyVersion,
