AwsCryptographicMaterialProviders/dafny/AwsCryptographyKeyStoreAdmin/src/KeyStoreAdminHelpers.dfy
@@ -1,0 +1,45 @@
+// Copyright Amazon.com Inc. or its affiliates. All Rights Reserved.
+// SPDX-License-Identifier: Apache-2.0
+include "../Model/AwsCryptographyKeyStoreAdminTypes.dfy"
+
+include "../../../dafny/AwsCryptographyKeyStore/src/KmsUtils.dfy"
+
+module {:options "/functionSyntax:4" } KeyStoreAdminHelpers {
+  import Types = AwsCryptographyKeyStoreAdminTypes
+  import KeyStoreTypes = AwsCryptographyKeyStoreTypes
+  import KmsArn
+  import KmsUtils
+  import KMS = Com.Amazonaws.Kms
+  
+  function KmsSymmetricKeyArnToKMSConfiguration(
+    kmsSymmetricArn: Types.KmsSymmetricKeyArn
+  ): (output: KeyStoreTypes.KMSConfiguration)
+    requires
+      match kmsSymmetricArn
+      case KmsKeyArn(arn) => KmsArn.ValidKmsArn?(arn)
+  {
+    match kmsSymmetricArn
+    case KmsKeyArn(kmsKeyArn) => KeyStoreTypes.kmsKeyArn(kmsKeyArn)
+  }
+  
+  datatype InternalSystemKey =
+    | TrustStorage()
+    | KmsSymEnc(
+        nameonly Tuple: KmsUtils.KMSTuple,
+        nameonly KeyId: KMS.Types.KeyIdType
+      )
+  {
+    ghost predicate ValidState()
+    {
+      match this
+      case TrustStorage() => true
+      case KmsSymEnc(Tuple, KeyId) =>
+        && Tuple.ValidState()
+        && KMS.Types.IsValid_KeyIdType(KeyId)
+        && Tuple.Modifies == Tuple.Modifies
+    }
+    ghost const Modifies := match this
+      case TrustStorage() => {}
+      case KmsSymEnc(Tuple, KeyId) => Tuple.Modifies
+  }
+}
