AwsCryptographicMaterialProviders/dafny/AwsCryptographyKeyStoreAdmin/src/SystemKey/Handler.dfy
@@ -2,7 +2,7 @@
 // SPDX-License-Identifier: Apache-2.0
 include "../../../AwsCryptographyKeyStore/src/HierarchicalVersionUtils.dfy"
 include "../../Model/AwsCryptographyKeyStoreAdminTypes.dfy"
-include "../KmsUtils.dfy"
+include "../KeyStoreAdminHelpers.dfy"
 include "ContentHandler.dfy"
 include "../CommitmentAndIndex.dfy"
 
@@ -17,7 +17,7 @@ module {:options "/functionSyntax:4" } SystemKey.Handler {
   import MPL = MaterialProviders
   import Types = AwsCryptographyKeyStoreAdminTypes
   import KSTypes = AwsCryptographyKeyStoreAdminTypes.AwsCryptographyKeyStoreTypes
-  import KmsUtils
+  import KeyStoreAdminHelpers
   import ContentHandler // = SystemKey.ContentHandler
   import HVUtils = HierarchicalVersionUtils
   import Structure
@@ -96,7 +96,7 @@ module {:options "/functionSyntax:4" } SystemKey.Handler {
   // TODO: Abstract and consolidate these 4 methods
   method SignCommitment(
     MutationCommitment: KSTypes.MutationCommitment,
-    InternalSystemKey: KmsUtils.InternalSystemKey
+    InternalSystemKey: KeyStoreAdminHelpers.InternalSystemKey
   ) returns (output: Result<KSTypes.MutationCommitment, Types.Error>)
     requires
       && InternalSystemKey.ValidState()
@@ -161,7 +161,7 @@ module {:options "/functionSyntax:4" } SystemKey.Handler {
 
   method SignIndex(
     MutationIndex: KSTypes.MutationIndex,
-    InternalSystemKey: KmsUtils.InternalSystemKey
+    InternalSystemKey: KeyStoreAdminHelpers.InternalSystemKey
   )
     returns (output: Result<KSTypes.MutationIndex, Types.Error>)
     requires
@@ -224,7 +224,7 @@ module {:options "/functionSyntax:4" } SystemKey.Handler {
 
   method VerifyCommitment(
     MutationCommitment: KSTypes.MutationCommitment,
-    InternalSystemKey: KmsUtils.InternalSystemKey
+    InternalSystemKey: KeyStoreAdminHelpers.InternalSystemKey
   ) returns (output: Result<bool, Types.Error>)
     requires
       && InternalSystemKey.ValidState()
@@ -292,7 +292,7 @@ module {:options "/functionSyntax:4" } SystemKey.Handler {
 
   method VerifyIndex(
     MutationIndex: KSTypes.MutationIndex,
-    InternalSystemKey: KmsUtils.InternalSystemKey
+    InternalSystemKey: KeyStoreAdminHelpers.InternalSystemKey
   ) returns (output: Result<bool, Types.Error>)
     requires
       && InternalSystemKey.ValidState()
